theories/typing/own.v
@@ -332,7 +332,7 @@ Section own.
     iSplit => //. by iFrame.
   Qed.
   Global Instance find_in_context_type_loc_own_inst l :
-    FindInContext (FindLoc l) 1%nat :=
+    FindInContext (FindLoc l) 1%nat FICSyntactic :=
     λ T, i2p (find_in_context_type_loc_own l T).
 
   Lemma find_in_context_type_val_own l T:
@@ -340,7 +340,7 @@ Section own.
     find_in_context (FindVal l) T.
   Proof. iDestruct 1 as (ty) "[Hl HT]". iExists _ => /=. by iFrame. Qed.
   Global Instance find_in_context_type_val_own_inst (l : loc) :
-    FindInContext (FindVal l) 1%nat :=
+    FindInContext (FindVal l) 1%nat FICSyntactic :=
     λ T, i2p (find_in_context_type_val_own l T).
 
   Lemma find_in_context_type_val_own_singleton (l : loc) T:
@@ -348,7 +348,7 @@ Section own.
     find_in_context (FindVal l) T.
   Proof. iIntros "[_ HT]". iExists _ => /=. iFrame "HT". simpl. done. Qed.
   Global Instance find_in_context_type_val_own_singleton_inst (l : loc):
-    FindInContext (FindVal l) 2%nat :=
+    FindInContext (FindVal l) 2%nat FICSyntactic :=
     λ T, i2p (find_in_context_type_val_own_singleton l T).
 
   (* We cannot use place here as it can easily lead to an infinite
@@ -361,7 +361,7 @@ Section own.
     find_in_context (FindValP l) T.
   Proof. rewrite /place'. iIntros "[_ HT]". iExists _. iFrame "HT" => //=. Qed.
   Global Instance find_in_context_type_val_P_own_singleton_inst (l : loc):
-    FindInContext (FindValP l) 2%nat :=
+    FindInContext (FindValP l) 2%nat FICSyntactic :=
     λ T, i2p (find_in_context_type_val_P_own_singleton l T).
 End own.
 Typeclasses Opaque place'.
